fix(LD_Issues): patch first part
change is_final from abbrev to definition

LD_Issues.thy
@@ -21,23 +21,23 @@ text\<open>Decode a pair of \<open>(l, x) \<in> \<nat> \<times> {0,1}*\<close> f
   Then, \<open>l\<close> is the number of leading \<open>1\<close>s.
   Remove all leading \<open>1\<close>s and one \<open>0\<close> to retain \<open>x\<close>.\<close>
 
-definition strip_sq_pad :: "word \<Rightarrow> word"
+definition strip_sq_pad :: "bool list \<Rightarrow> bool list"
   where "strip_sq_pad w \<equiv> drop (suffix_len w) w"
 
-definition decode_pair_l :: "word \<Rightarrow> nat"
+definition decode_pair_l :: "bool list \<Rightarrow> nat"
   where "decode_pair_l w = length (takeWhile (\<lambda>x. x = True) (rev (strip_sq_pad w)))"
 
-definition decode_pair_x :: "word \<Rightarrow> word"
+definition decode_pair_x :: "bool list \<Rightarrow> bool list"
   where "decode_pair_x w = rev (tl (dropWhile (\<lambda>x. x = True) (rev (strip_sq_pad w))))"
 
-abbreviation decode_pair :: "word \<Rightarrow> nat \<times> word"
+abbreviation decode_pair :: "bool list \<Rightarrow> nat \<times> bool list"
   where "decode_pair w \<equiv> (decode_pair_l w, decode_pair_x w)"
 
 
-definition rev_suffix_len :: "word \<Rightarrow> nat"
+definition rev_suffix_len :: "bool list \<Rightarrow> nat"
   where "rev_suffix_len w = length w + 9"
 
-definition encode_pair :: "nat \<Rightarrow> word \<Rightarrow> word"
+definition encode_pair :: "nat \<Rightarrow> bool list \<Rightarrow> bool list"
   where "encode_pair l x = (let w' = x @ [False] @ True \<up> l in
             False \<up> (rev_suffix_len w') @ w')"
 
@@ -59,14 +59,17 @@ proof -
     unfolding w encode_pair_def Let_def w'[symmetric] by simp
 qed
 
-lemma decode_encode_pair:
+lemma decode_encode_pair[simp]:
   fixes l x
   defines w: "w \<equiv> encode_pair l x"
-  shows "decode_pair w = (l, x)"
-proof (unfold prod.inject, intro conjI)
+  shows decode_encode_pair_l: "decode_pair_l w = l"
+    and decode_encode_pair_x: "decode_pair_x w = x"
+    (* and decode_encode_pair_: "decode_pair w = (l, x)" *)
+proof -
   have rw: "rev (strip_sq_pad w) = True \<up> l @ False # rev x" unfolding w strip_sq_pad_pair by force
-  show "decode_pair_l w = l" unfolding decode_pair_l_def rw by (subst takeWhile_tail) auto
-  show "decode_pair_x w = x" unfolding decode_pair_x_def rw by (subst dropWhile_append3) auto
+  show l: "decode_pair_l w = l" unfolding decode_pair_l_def rw by (subst takeWhile_tail) auto
+  show x: "decode_pair_x w = x" unfolding decode_pair_x_def rw by (subst dropWhile_append3) auto
+  (* from l x show "decode_pair w = (l, x)" by (fact arg_cong2) *)
 qed
 
 
@@ -101,40 +104,40 @@ text\<open>Note: this is not intended to replace \<^const>\<open>L\<^sub>D\<clos
   to prove properties of \<open>L\<^sub>D''\<close> via reduction to \<open>L\<^sub>D\<close>.
 
   Construction: Given a word \<open>w\<close>.
-  Split the word \<open>w\<close> into \<open>(l::nat, x::word)\<close> using \<^const>\<open>decode_pair\<close>.
+  Split the word \<open>w\<close> into \<open>(l::nat, x::bool list)\<close> using \<^const>\<open>decode_pair\<close>.
   Define \<open>v\<close> as the \<open>l\<close> most-significant-bits of \<open>x\<close>.
   Remove the arbitrary-length \<open>1\<^sup>+0\<close>-prefix from \<open>v\<close> to retain the pure encoding of \<open>M\<^sub>v\<close>.
   If \<open>M\<^sub>v\<close> rejects \<open>v\<close> within \<open>T(len(x))\<close> steps, \<open>w \<in> L\<^sub>D''\<close> holds.
 
-  Note that in this version, using \<^const>\<open>time_bounded_word\<close> is not possible,
+  Note that in this version, using \<^const>\<open>TM.time_bounded_word\<close> is not possible,
   as the word that determines the time bound (\<open>x\<close>) differs from the input word (\<open>v\<close>).
-  The alternative version shown in @{thm time_bounded_altdef} is used for simplicity.\<close>
+  The alternative version shown in @{thm TM.time_bounded_altdef2} is used for simplicity.\<close>
 
-definition L\<^sub>D'' :: lang
-  where "L\<^sub>D'' \<equiv> {w.
+definition L\<^sub>D'' :: "bool lang"
+  where "L\<^sub>D'' \<equiv> Lang UNIV (\<lambda>w.
       let (l, x) = decode_pair w;
           v = drop (length x - l) x;
-          M\<^sub>v = TM_decode_pad v in
-      rejects M\<^sub>v v \<and> is_final (steps0 (1, <v>\<^sub>t\<^sub>p) M\<^sub>v (tcomp\<^sub>w T x))
-    }"
+          M\<^sub>v = dec_TM_pad v in
+      TM.rejects M\<^sub>v v \<and> TM.is_final M\<^sub>v (TM.run M\<^sub>v (T (length x)) v)
+    )"
 
-definition L\<^sub>0'' :: lang
-  where "L\<^sub>0'' \<equiv> L\<^sub>D'' \<inter> SQ"
+definition L\<^sub>0'' :: "bool lang"
+  where "L\<^sub>0'' \<equiv> L\<^sub>D'' \<inter>\<^sub>L SQ"
 
 
 lemma L\<^sub>D''_adj_sq_iff:
   fixes w
-  defines w': "w' \<equiv> adj_sq\<^sub>w w"
+  defines "w' \<equiv> adj_sq\<^sub>w w"
   assumes len: "length w \<ge> 9"
-  shows "w' \<in> L\<^sub>D'' \<longleftrightarrow> w \<in> L\<^sub>D''"
-  unfolding L\<^sub>D''_def mem_Collect_eq w' len[THEN pair_adj_sq_eq] ..
+  shows "w' \<in>\<^sub>L L\<^sub>D'' \<longleftrightarrow> w \<in>\<^sub>L L\<^sub>D''"
+  unfolding L\<^sub>D''_def words_simp mem_Collect_eq w'_def pair_adj_sq_eq[OF len] by blast
 
 lemma L\<^sub>D''_L\<^sub>0''_adj_sq_iff:
   fixes w
-  defines w': "w' \<equiv> adj_sq\<^sub>w w"
+  defines "w' \<equiv> adj_sq\<^sub>w w"
   assumes len: "length w \<ge> 9"
-  shows "w' \<in> L\<^sub>0'' \<longleftrightarrow> w \<in> L\<^sub>D''"
-  unfolding L\<^sub>0''_def w' using len[THEN L\<^sub>D''_adj_sq_iff] adj_sq_word_correct by blast
+  shows "w' \<in>\<^sub>L L\<^sub>0'' \<longleftrightarrow> w \<in>\<^sub>L L\<^sub>D''"
+  unfolding L\<^sub>0''_def w'_def using L\<^sub>D''_adj_sq_iff[OF len] adj_sq_word_correct by simp
 
 
 subsection\<open>\<open>L\<^sub>D'' \<notin> DTIME(t)\<close> via Reduction from \<open>L\<^sub>D\<close> to \<open>L\<^sub>D''\<close>\<close>
@@ -144,7 +147,7 @@ text\<open>Reduce \<open>L\<^sub>D\<close> to \<open>L\<^sub>D''\<close>:
     Decoding \<open>w'\<close> then yields \<open>(l, w)\<close> which results in the intermediate value \<open>v\<close>
     being equal to \<open>w\<close> in the definition of \<^const>\<open>L\<^sub>D''\<close>.\<close>
 
-definition reduce_LD_LD'' :: "word \<Rightarrow> word"
+definition reduce_LD_LD'' :: "bool list \<Rightarrow> bool list"
   where "reduce_LD_LD'' w \<equiv> encode_pair (length w) w"
 
 lemma reduce_LD_LD''_len: "length (reduce_LD_LD'' w) = 4 * length w + 11"
@@ -152,14 +155,20 @@ lemma reduce_LD_LD''_len: "length (reduce_LD_LD'' w) = 4 * length w + 11"
 
 lemma reduce_LD_LD''_correct:
   fixes w
-  defines w'': "w'' \<equiv> reduce_LD_LD'' w"
-  shows "w'' \<in> L\<^sub>D'' \<longleftrightarrow> w \<in> L\<^sub>D"
+  defines [simp]: "w'' \<equiv> reduce_LD_LD'' w"
+  shows "w'' \<in>\<^sub>L L\<^sub>D'' \<longleftrightarrow> w \<in>\<^sub>L L\<^sub>D"
 proof -
-  let ?M\<^sub>w = "TM_decode_pad w"
-  have "w'' \<in> L\<^sub>D'' \<longleftrightarrow> rejects ?M\<^sub>w w \<and> time_bounded_word T ?M\<^sub>w w"
-    unfolding L\<^sub>D''_def w'' reduce_LD_LD''_def mem_Collect_eq decode_encode_pair
-    unfolding diff_self_eq_0 drop_0 Let_def prod.case unfolding time_bounded_altdef ..
-  also have "... \<longleftrightarrow> w \<in> L\<^sub>D" unfolding LD_def mem_Collect_eq Let_def ..
+  let ?M\<^sub>w = "dec_TM_pad w"
+  interpret TM ?M\<^sub>w .
+
+  have *: "(let (l, x) = decode_pair w'';
+                  v = drop (length x - l) x;
+                 M\<^sub>v = dec_TM_pad v in P M\<^sub>v x v) \<longleftrightarrow> P ?M\<^sub>w w w" for P
+    unfolding w''_def reduce_LD_LD''_def decode_encode_pair Let_def prod.case by simp
+
+  have "w'' \<in>\<^sub>L L\<^sub>D'' \<longleftrightarrow> rejects w \<and> time_bounded_word T w"
+    unfolding L\<^sub>D''_def member_lang_UNIV mem_Collect_eq * TM.time_bounded_word_def ..
+  also have "... \<longleftrightarrow> w \<in>\<^sub>L L\<^sub>D" by (simp add: L\<^sub>D_def Let_def)
   finally show ?thesis .
 qed
 
@@ -256,7 +265,7 @@ proof (rule ccontr, unfold not_not)
   proof (rule reduce_DTIME)
     show "almost_everywhere (\<lambda>w. (adj_sq\<^sub>w w \<in> L\<^sub>0'') = (w \<in> L\<^sub>D'') \<and> length (adj_sq\<^sub>w w) \<le> length w)"
     proof (intro ae_word_lengthI exI allI impI conjI)
-      fix w :: word assume len: "length w \<ge> 9"
+      fix w :: "bool list" assume len: "length w \<ge> 9"
       from len show "adj_sq\<^sub>w w \<in> L\<^sub>0'' \<longleftrightarrow> w \<in> L\<^sub>D''" by (fact L\<^sub>D''_L\<^sub>0''_adj_sq_iff)
       from len show "length (adj_sq\<^sub>w w) \<le> length w"
         by (intro eq_imp_le sh_msbD) (fact adj_sq_sh_pfx_half)
